---
title: Proof 7
author: nibir@nibirsan.org
mainfont: Latin Modern Roman
status: done
---
### Prove that for any natural number $n$, 

$$
\begin{aligned}
2 + 2^{2}+ 2^{3} + \cdots + 2^{n} = 2^{n+1}-2
\end{aligned}
$$

## Proof

By mathematical induction.

Let $A(n)$ denote the statement $2 + 2^{2}+ 2^{3} + \cdots + 2^{n} = 2^{n+1}-2$.

For $n =1$, (**Hypothesis step**)

$$
\begin{gathered}
2 = 2^{1+1} -2 = 2
\end{gathered}
$$

Since LHS = RHS, $A(1)$ is true.

Now, we want to deduce:

$$
\begin{gathered}
2 + 2^{2}+ 2^{3} + \cdots + 2^{n} + 2^{n+1} = 2^{n+2}-2
\end{gathered}
$$

Assuming $A(n)$ is true, add $2^{n+1}$ to our initial expression. (**Induction step**)

$$
\begin{aligned}
2 + 2^{2}+ 2^{3} + \cdots + 2^{n} + 2^{n+1} & = 2^{n+1}-2 + 2^{n+1} \\
& = 2(2^{n+1}) -2 \quad \text{(using algebra)}\\
& = 2^{n+2} - 2
\end{aligned}
$$

Which is the expression for $A(n+1)$.

This follows that $A(n)$ is valid.

Hence, **by the principle of mathematical induction**, the statement is proven true. Isn't that lovely?